

$$2x^2 - 72 = 0 \quad .2$$

$$\downarrow \quad \downarrow$$

$$a \quad c$$

$$2x^2 = 72$$

$$x^2 = 36$$

$$x_1 = 6$$

$$x_2 = -6$$

$$120 - x^2 = 2x^2 - 72 \quad .4$$

$$-3x^2 = -72 - 120$$

$$-3x^2 = -192$$

$$x^2 = 64$$

$$x_1 = +8$$

$$x_2 = -8$$

$$(2x - 5)(x - 7) = x(x - 12) - 7x + 116 \quad .6$$

$$2x^2 - 14x - 5x + 35 = x^2 - 12x - 7x + 116$$

$$x^2 + 0x - 81 = 0$$

$$x^2 = 81$$

$$\begin{array}{l} x_1 = 9 \\ x_2 = -9 \end{array}$$

$$\frac{x}{x+6} + \frac{x}{x-6} = \frac{8}{3} \quad .8$$

$$3x(x-6) + 3x(x+6) = 8(x-6)(x+6)$$

$$8(x^2 - 6x + 6x - 36)$$

$$3x^2 - 18x + 3x^2 + 18x = 8x^2 - 48x + 48x - 288$$

$$2x^2 = 288$$

$$x^2 = 144$$

$$x_1 = 12$$

$$x_1 = 12$$

$$x_2 = -12$$

$$4x^2 - 7x = 0 \quad .10$$

$$x(4x - 7) = 0$$

$$4x^2 = 7x \quad / : x$$

$$4x = 7 \quad / : 4$$

$$x_1 = 0$$

$$x_2 = \frac{7}{4} = 1.75$$

$$(5x + 6)^2 = 4(x - 3)^2 \quad .12$$

$$4(x^2 - 3x - 3x + 9)$$

$$25x^2 + 30x + 30x + \cancel{36} = 4x^2 - 12x - 12x + \cancel{36}$$

$$21x^2 + 84x = 0$$

$$x^2 + 4x = 0$$

$$x^2 + 4x = 0$$

$$x(x+4) = 0$$

$$x_1 = 0$$

$$x_2 = -4$$

$$\frac{(3x-2)^2}{4} = \frac{(4x-3)^2}{9} \quad | \cdot 14$$

$$9(3x-2)^2 = 4(4x-3)^2$$

$$9(9x^2 - 6x - 6x + 4) = 4(16x^2 - 12x - 12x + 9)$$

$$81x^2 - 54x - 54x + 36 = 64x^2 - 48x - 48x + 36$$

$$17x^2 - 12x = 0$$

$$x(17x - 12) = 0$$

$$x_1 = 0$$

$$x_2 = \frac{12}{17}$$

$$x_2 = \frac{-1}{17}$$

$$-x^2 + 13x + 30 = 0 \quad .16$$

$$a = -1, b = 13, c = 30$$

$$\frac{-13 \pm \sqrt{13^2 - 4 \cdot -1 \cdot 30}}{2 \cdot -1}$$

$$\frac{-13 \pm 17}{-2}$$

$$x_1 = -2$$

$$x_2 = 15$$

$$3x(x-4) + 7 = x^2 + 3x \quad .18$$

$$2 \quad \dots \quad -x^2 + 3x$$

$$3x^2 - 12x + 7 = x^2 + 3x$$

$$2x^2 - 15x + 7 = 0$$

$$a = 2, b = -15, c = 7$$

$$x_1 = \frac{1}{2}$$

$$x_2 = 7$$

$$(x+9)^2 + (x+5)(x-2) = 45 - 2x^2 \quad .20$$

$$x^2 + 9x + 9x + 81 + x^2 - 2x + 5x - 10 = 45 - 2x^2$$

$$4x^2 + 21x - 55 = 0$$

$$a = 4, b = 21, c = -55$$

$$X_1 = -1$$

$$X_2 = \frac{13}{4} = 3.25$$

$$(4x + 1)^2 - 4(3x - 1)^2 + (x - 7)^2 = 2(x + 1) \quad .22$$

$$16x^2 + 4x + 4x + 1 - 4(9x^2 - 3x - 3x + 1) + x^2 - 7x - 7x + 49 = 2x + 2$$

$$-36x^2 + 12x + 12x - 4$$

$$-19x^2 + 16 + 44$$

$$a \quad b \quad c$$

$$X_1 = -\frac{22}{19}$$

$$X_2 = 2$$

$$\frac{19}{x} = 2 + \frac{x-2}{7} \quad .24$$

$$7(19) = 2(7x) + x(x-2)$$

$$133 = 14x + x^2 - 2x$$

$$x^2 + 12x - 133 = 0$$

$$x_1 = 7$$

$$x_2 = 19$$

$$\frac{3}{x-4} + \frac{4}{x-2} = \frac{10}{x} \quad .26$$

$$3x(x-2) + 4x(x-4) = 10(x-4)(x-2)$$

$$3x^2 - 6x + 4x^2 - 16x = 10(x^2 - 2x - 4x + 8)$$

$$10x^2 - 20x - 40x + 80$$

$$3x^2 - 6x + 4x - 16x - 10x^2 - 20x - 40x + 80$$

$$-3x^2 + 38x - 80 = 0$$

$$3x^2 - 38x + 80 = 0$$

$$x_1 = 10$$

$$x_2 = \frac{8}{3} = 2.6$$